Progress and bugfixes

ecoop17/dot_storeless_wfrel.v
@@ -13,15 +13,14 @@ Require Import tactics.
 (*******************)
 (* Renames for adaption. *)
 
-Definition tsize_flat := tsize.
+Notation tsize_flat := tsize.
 
 Lemma open_preserves_size': forall T v j,
     tsize_flat (open j v T) = tsize_flat T.
-Proof. unfold tsize_flat; intros; rewrite <- open_preserves_size; easy. Qed.
+Proof. intros; rewrite <- open_preserves_size; easy. Qed.
 Definition vl := tm.
 
 Definition closed_ty i j T := closed j i T.
-Definition wf {A} (G : list A) T := closed_ty 0 (length G) T.
 
 (*******************)
 (* Small-step semantics *)
@@ -106,7 +105,7 @@ Ltac smaller_n :=
 Ltac smaller_types :=
   Tactics.program_simpl;
   autounfold; apply right_lex;
-  unfold open; try rewrite <- open_preserves_size;
+  try rewrite open_preserves_size';
   (* simpl; omega. *)
   simple_ineq.
 
@@ -184,9 +183,10 @@ Equations expr_sem n (T : ty) (A : pretype_dom n) k (p : k <= n) (t : tm) : Prop
 Equations val_type (Tn: ty * nat) (v : tm) : Prop :=
   val_type Tn t by rec Tn val_type_termRel :=
     val_type (pair TBot n) v := False;
-    val_type (pair TTop n) v := True;
+    val_type (pair TTop n) v := irred v /\ tm_closed 0 0 v;
     val_type (pair (TFun l T1 T2) n) (tvar (VObj ds)) :=
-                                  closed_ty 0 0 T1 /\ closed_ty 1 0 T2 /\
+                                  closed 0 0 T1 /\ closed 0 1 T2 /\
+                                  dms_closed 0 1 ds /\
                                   exists U1 U2 t,
                                     index l (dms_to_list (subst_dms ds ds)) = Some (dfun U1 U2 t) /\
                                     (forall vyds k (Hj: k < n),
@@ -194,16 +194,18 @@ Equations val_type (Tn: ty * nat) (v : tm) : Prop :=
                                         expr_sem k
                                           (open 0 (VObj vyds) T2)
                                           (fun kj p t => val_type (open 0 (VObj vyds) T2, kj) t)
-                                          k _ t);
+                                          k _ (subst_tm vyds t));
     val_type (pair (TMem l L U) n) (tvar (VObj ds)) :=
-                                       closed_ty 0 0 L /\ closed_ty 0 0 U /\
+                                       closed_ty 0 0 L /\ closed_ty 0 0 U /\ dms_closed 0 1 ds /\
                                        exists TX, index l (dms_to_list (subst_dms ds ds)) = Some (dty TX) /\
                                              (forall vy j (Hj: j <= n), val_type (pair L j) vy -> val_type (pair U j) vy) /\
                                              (forall vy j (Hj: j < n),
                                                  (val_type (pair L j) vy -> val_type (pair TX j) vy) /\
                                                  (val_type (pair TX j) vy -> val_type (pair U j) vy));
     val_type (pair (TSel (VObj ds) l) n) v :=
+                                         irred v /\
                                          dms_closed 0 1 ds /\
+                                         tm_closed 0 0 v /\
                                          exists TX, index l (dms_to_list (subst_dms ds ds)) = Some (dty TX) /\
                                                forall j (Hj: j < n), val_type (TX, j) v;
     val_type (pair (TBind T) n) (tvar (VObj ds)) :=
@@ -232,17 +234,71 @@ Defined.
 
 Definition vtp T n v := val_type (T, n) v.
 Hint Unfold vtp.
-Example ex0 : forall n v, vtp TTop n v.
+Example ex0 : forall n v, irred v -> tm_closed 0 0 v -> vtp TTop n v.
 Proof.
   intros; autounfold; now simp val_type.
 Qed.
 
-Hint Constructors closed.
+Lemma vtp_irred: forall T k v, vtp T k v -> irred v.
+Proof.
+  intros *; unfold vtp in *;
+    funind (val_type (T, k) v) Hcall; intros; ev;
+      solve [easy | intuition auto | unfold irred; intro Hsteps; ev; easy ].
+Qed.
+Hint Resolve vtp_irred.
+
 Hint Unfold closed_ty.
-Example ex3: forall T n, vtp (TMem 0 TBot TTop) n (tvar (VObj (dcons (dty T) dnil))).
+Hint Constructors vr_closed.
+Hint Constructors closed.
+Hint Constructors dms_closed.
+Hint Constructors dm_closed.
+Hint Constructors tm_closed.
+Hint Constructors dm_closed.
+
+Lemma vtp_closed: forall T n v,
+    vtp T n v -> closed_ty 0 0 T.
+Proof.
+  unfold vtp, closed_ty;
+    intros *; vtp_induction T n; intros;
+      destruct T;
+      destruct v;
+      simp val_type in *; ev;
+        try eauto || easy.
+  all: (destruct v0 || destruct v; simp val_type in *; ev; now eauto)
+       || constructor; eapply H; smaller_types.
+Qed.
+
+Lemma vtp_v_closed : forall T n v, vtp T n v -> tm_closed 0 0 v.
+  (* unfold vtp; intros; remember H as Hvtp; funind (val_type (T, n) v) Hcall; simp val_type in *. *)
+  (* - admit. *)
+  (* - ev; clear Hcall. simp expr_sem in *. *)
+  (*   admit. *)
+  unfold vtp;
+    intros *; vtp_induction T n; intros * Hind; intros;
+    destruct T;
+    destruct v;
+    simp val_type in *; ev;
+      try eauto || easy.
+  all: try solve [destruct v; simp val_type in *; ev; now eauto].
+  all: try solve [destruct v0; simp val_type in *; ev; now eauto].
+  all: try (destruct v0; simp val_type in *; ev; eauto).
+  Ltac indSearch Hind :=
+    match goal with
+    | H : val_type (?T1, ?n1) _ |- _ =>
+      lets ?: Hind H; smaller_types
+    end.
+  all: try indSearch Hind.
+  all: try (match goal with
+    | H : ?A \/ ?B |- _ => destruct H
+    end; indSearch Hind).
+  - destruct v; simp val_type in *; ev; eauto; indSearch Hind.
+Qed.
+Hint Resolve vtp_v_closed.
+
+Example ex3: forall T n, closed 0 1 T -> vtp (TMem 0 TBot TTop) n (tvar (VObj (dcons (dty T) dnil))).
 Proof.
   intros; autounfold; simp val_type; intuition eauto; simpl;
-  eexists; intuition eauto; now simp val_type in *.
+    eexists; intuition eauto; simp val_type in *; eauto; try easy.
 Qed.
 
 (* (* Check syntax_mutind. *) *)
@@ -266,22 +322,8 @@ Qed.
 (* (*   (* repeat better_case_match; try constructor; inverts H. *) *) *)
 (* (* Admitted. *) *)
 
-Hint Constructors vr_closed.
-Hint Constructors dms_closed.
 (* Hint Extern 100 (val_type_termRel _ _) => *)
 (*   valTypeObligationsSSReflection. *)
-Lemma vtp_closed: forall T n v,
-    vtp T n v -> closed_ty 0 0 T.
-Proof.
-  unfold vtp, closed_ty;
-  intros *; vtp_induction T n; intros;
-    destruct T;
-    destruct v;
-    simp val_type in *; ev;
-      try eauto || easy.
-  all: (destruct v0 || destruct v; simp val_type in *; ev; now eauto) ||
-           constructor; eapply H; smaller_types.
-Qed.
   (* (* all: try solve [destruct v; simp val_type in *; ev; now eauto]. *) *)
   (* (* all: try solve *) *)
   (* (*       [ destruct v; simp val_type in *; ev; now eauto | *) *)
@@ -319,6 +361,7 @@ Qed.
   (* (*   repeat better_case_match; ev; eauto 6; *) *)
   (* (*     contradiction. *) *)
 
+
 Lemma vtp_mon: forall T v m n,
     vtp T n v ->
     m <= n ->
@@ -332,11 +375,13 @@ Proof.
     simp expr_sem in *;
     repeat split_conj; eauto; try easy.
 
-  - do 3 eexists; split_conj; eauto; intros;
-    lets Hfunsucceeds: H3 ___; eauto.
+  - do 3 eexists; split_conj; eauto; intros.
+    match goal with
+    | Hfun: forall (ds: dms), _ |- _ =>
+      lets Hfunsucceeds: Hfun ___; eauto
+    end.
     Unshelve.
     omega.
-
   - eexists; split_conj; eauto.
 
   - match goal with
@@ -411,15 +456,7 @@ Proof.
   intros * H; induction H; simpl; congruence.
 Qed.
 
-Program Definition etp0 T k e :=
-  expr_sem k T (fun k _ => vtp T k) k _ e.
-
-Lemma etp0_closed: forall T k v,
-    etp0 T k v -> closed_ty 0 0 T.
-Proof.
-  unfold etp0; intros; simp expr_sem in *; tauto.
-Qed.
-Hint Resolve etp0_closed.
+Hint Constructors Forall.
 
 (* Fixpoint subst_all_ty (env : venv) (T: ty) := *)
 (*   match env with *)
@@ -436,47 +473,524 @@ Hint Resolve etp0_closed.
 (*   easy. *)
 (* Qed. *)
 
-Require Import dot_monads.
-Fixpoint vr_subst_all (env: list vr) (v: vr) { struct v }: vr :=
+(* Require Import dot_monads. *)
+
+(* Fixpoint vr_subst_all (env: list vr) (v: vr) { struct v }: option vr := *)
+(*   match v with *)
+(*     | VarF x => ret (VarF x) *)
+(*     | VarB x => index x env *)
+(*     | VObj dms => *)
+(*       dms' <- dms_subst_all (VarB 0 :: env) dms; *)
+(*       ret (VObj dms') *)
+(*   end *)
+(* with subst_all (env: list vr) (T: ty) { struct T }: option ty := *)
+(*   match T with *)
+(*     | TTop        => ret TTop *)
+(*     | TBot        => ret TBot *)
+(*     | TSel v1 l     => *)
+(*       v1' <- vr_subst_all env v1; *)
+(*       ret (TSel v1' l) *)
+(*     | TFun l T1 T2  => *)
+(*       T1' <- subst_all env T1; *)
+(*       T2' <- subst_all (VarB 0 :: env) T2; *)
+(*       ret (TFun l T1' T2') *)
+(*     | TMem l T1 T2  => *)
+(*       T1' <- subst_all env T1; *)
+(*       T2' <- subst_all env T2; *)
+(*       ret (TMem l T1' T2') *)
+(*     | TBind T1    => *)
+(*       T1' <- subst_all (VarB 0 :: env) T1; *)
+(*       ret (TBind T1') *)
+(*     | TAnd T1 T2  => *)
+(*       T1' <- subst_all env T1; *)
+(*       T2' <- subst_all env T2; *)
+(*       ret (TAnd T1' T2') *)
+(*     | TOr T1 T2   => *)
+(*       T1' <- subst_all env T1; *)
+(*       T2' <- subst_all env T2; *)
+(*       ret (TOr T1' T2') *)
+(*   end *)
+(* with tm_subst_all (env: list vr) (t: tm) { struct t }: option tm := *)
+(*    match t with *)
+(*      | tvar v => v' <- vr_subst_all env v; ret (tvar v') *)
+(*      | tapp t1 l t2 => *)
+(*        t1' <- tm_subst_all env t1; *)
+(*        t2' <- tm_subst_all env t2; *)
+(*        ret (tapp t1' l t2') *)
+(*    end *)
+(* with dm_subst_all (env: list vr) (d: dm) { struct d }: option dm := *)
+(*    match d with *)
+(*      | dfun T1 T2 t2 => *)
+(*        T1' <- subst_all env T1; *)
+(*        T2' <- subst_all (VarB 0 :: env) T2; *)
+(*        t2' <- tm_subst_all (VarB 0 :: env) t2; *)
+(*        ret (dfun T1' T2' t2') *)
+(*      | dty T1 => *)
+(*        T1' <- subst_all env T1; *)
+(*        ret (dty T1') *)
+(*    end *)
+(* with dms_subst_all (env: list vr) (ds: dms) { struct ds }: option dms := *)
+(*    match ds with *)
+(*      | dnil => ret dnil *)
+(*      | dcons d ds => *)
+(*        d'  <- dm_subst_all env d; *)
+(*        ds' <- dms_subst_all env ds; *)
+(*        ret (dcons d' ds') *)
+(*    end. *)
+
+Ltac beq_nat :=
+  match goal with
+  | H : (?a =? ?b) = true |- _ => try eapply beq_nat_true in H
+  | H : (?a =? ?b) = false |- _ => try eapply beq_nat_false in H
+  end.
+
+Lemma index_Forall:
+  forall {X} (env : list X) i P, Forall P env -> i < length env ->
+                            exists v, index i env = Some v /\ P v.
+Proof.
+  intros * HFor Hlen; induction env.
+  - easy.
+  - inverse HFor; simpl; case_match; beq_nat; eauto.
+Qed.
+
+(* (* SearchPattern ((?A -> Prop) -> list ?A -> Prop). *) *)
+(* Lemma subst_all_closed_upgrade_rec_vr: *)
+(*   forall env i, *)
+(*     Forall (vr_closed i 0) env -> *)
+(*     forall j v, *)
+(*       vr_closed i j v -> length env = j -> *)
+(*       exists v', vr_subst_all env v = Some v' /\ *)
+(*             vr_closed i 0 v'. *)
+(* Proof. *)
+(*   intros * HenvCl; induction v; intros * Hcl Hlen; simpl in *; inverse Hcl; *)
+(*   intuition eauto using index_Forall. *)
+(* Abort. *)
+
+(* Lemma subst_all_closed_upgrade_rec: *)
+(*   (forall v, forall i k env, Forall (vr_closed i k) env -> forall j, vr_closed i j v -> length env = j -> exists v', vr_subst_all env v = Some v' /\ vr_closed i k v') /\ *)
+(*   (forall T, forall i k env, Forall (vr_closed i k) env -> forall j, closed i j T -> length env = j -> exists T', subst_all env T = Some T' /\ closed i k T') /\ *)
+(*   (forall t, forall i k env, Forall (vr_closed i k) env -> forall j, tm_closed i j t -> length env = j -> exists t', tm_subst_all env t = Some t' /\ tm_closed i k t') /\ *)
+(*   (forall dm, forall i k env, Forall (vr_closed i k) env -> forall j, dm_closed i j dm -> length env = j -> exists dm', dm_subst_all env dm = Some dm' /\ dm_closed i k dm') /\ *)
+(*   (forall T, forall i k env, Forall (vr_closed i k) env -> forall j, dms_closed i j T -> length env = j -> exists dms', dms_subst_all env T = Some dms' /\ dms_closed i k dms'). *)
+(* Proof. *)
+(*   apply syntax_mutind. *)
+(*   all: try solve [intros * HenvCl * Hcl * Hlen; simpl in *; inverse Hcl; simpl in *; subst; intuition eauto using index_Forall]. *)
+(*   - intros * Hind * HenvCl * Hcl * Hlen; simpl in *; inverts Hcl. *)
+
+(*     Ltac indLater Hind env i j k :=  *)
+(*       lets (? & -> & ?): Hind i (S k) (VarB 0 :: env) (S j) ___; simpl; eauto; *)
+(*       try (constructors; [eauto | eapply Forall_impl with (P := vr_closed i k); intuition eauto using (proj1 closed_upgrade_rec)]). *)
+(*     indLater Hind env i j k. *)
+(*   - intros * Hindt * Hindt1 * HenvCl * Hcl * Hlen; simpl in *; inverts Hcl. *)
+(*     Ltac indNow Hind env i j k :=  *)
+(*       lets (? & -> & ?): Hind i k env j ___; simpl; eauto. *)
+(*     indNow Hindt env i j k. *)
+(*     indLater Hindt1 env i j k. *)
+(*   - intros * Hindt * Hindt1 * HenvCl * Hcl * Hlen; simpl in *; inverts Hcl. *)
+(*     indNow Hindt env i j k. *)
+(*     indNow Hindt1 env i j k. *)
+(*   - intros * Hindt * HenvCl * Hcl * Hlen; simpl in *; inverts Hcl. *)
+(*     indNow Hindt env i j k. *)
+(*   - intros * Hindt * HenvCl * Hcl * Hlen; simpl in *; inverts Hcl. *)
+(*     indLater Hindt env i j k. *)
+(*   - intros * Hindt * Hindt1 * HenvCl * Hcl * Hlen; simpl in *; inverts Hcl. *)
+(*     indNow Hindt env i j k. *)
+(*     indNow Hindt1 env i j k. *)
+(*   - intros * Hindt * Hindt1 * HenvCl * Hcl * Hlen; simpl in *; inverts Hcl. *)
+(*     indNow Hindt env i j k. *)
+(*     indNow Hindt1 env i j k. *)
+(*   - intros * Hindt * HenvCl * Hcl * Hlen; simpl in *; inverts Hcl. *)
+(*     indNow Hindt env i j k. *)
+(*   - intros * Hindt * Hindt1 * HenvCl * Hcl * Hlen; simpl in *; inverts Hcl. *)
+(*     indNow Hindt env i j k. *)
+(*     indNow Hindt1 env i j k. *)
+(*   - intros * Hindt * Hindt1 * Hindt2 * HenvCl * Hcl * Hlen; simpl in *; inverts Hcl. *)
+(*     indNow Hindt env i j k. *)
+(*     indLater Hindt1 env i j k. *)
+(*     indLater Hindt2 env i j k. *)
+(*   - intros * Hindt * HenvCl * Hcl * Hlen; simpl in *; inverts Hcl. *)
+(*     indNow Hindt env i j k. *)
+(*   - intros * Hindt * Hindt1 * HenvCl * Hcl * Hlen; simpl in *; inverts Hcl. *)
+(*     indNow Hindt env i j k. *)
+(*     indNow Hindt1 env i j k. *)
+(* Qed. *)
+
+(* Lemma subst_all_success_rec: *)
+(*   (forall v, forall i env, forall j, vr_closed i j v -> length env = j -> exists v', vr_subst_all env v = Some v') /\ *)
+(*   (forall T, forall i env, forall j, closed i j T -> length env = j -> exists T', subst_all env T = Some T') /\ *)
+(*   (forall t, forall i env, forall j, tm_closed i j t -> length env = j -> exists t', tm_subst_all env t = Some t') /\ *)
+(*   (forall dm, forall i env, forall j, dm_closed i j dm -> length env = j -> exists dm', dm_subst_all env dm = Some dm') /\ *)
+(*   (forall T, forall i env, forall j, dms_closed i j T -> length env = j -> exists dms', dms_subst_all env T = Some dms'). *)
+(* Proof. *)
+(*   apply syntax_mutind. *)
+(*   all: try solve [intros * Hcl * Hlen; simpl in *; inverse Hcl; simpl in *; subst; intuition eauto using index_Forall]. *)
+(*   - intros * Hcl * Hlen; simpl in *; inverts Hcl. apply index_exists; auto. *)
+(*     Ltac indNow' Hind env i j := *)
+(*       lets (? & ->): Hind i env j ___; simpl; eauto. *)
+(*     Ltac indLater' Hind env i j := *)
+(*       lets (? & ->): Hind i (VarB 0 :: env) (S j) ___; simpl; eauto. *)
+
+(*   - intros * Hindt * Hcl * Hlen; simpl in *; inverts Hcl. *)
+(*     indLater' Hindt env i j. *)
+(*   - intros * Hindt * Hindt1 * Hcl * Hlen; simpl in *; inverts Hcl. *)
+(*     indNow' Hindt env i j. *)
+(*     indLater' Hindt1 env i j. *)
+(*   - intros * Hindt * Hindt1 * Hcl * Hlen; simpl in *; inverts Hcl. *)
+(*     indNow' Hindt env i j. *)
+(*     indNow' Hindt1 env i j. *)
+(*   - intros * Hindt * Hcl * Hlen; simpl in *; inverts Hcl. *)
+(*     indNow' Hindt env i j. *)
+(*   - intros * Hindt * Hcl * Hlen; simpl in *; inverts Hcl. *)
+(*     indLater' Hindt env i j. *)
+(*   - intros * Hindt * Hindt1 * Hcl * Hlen; simpl in *; inverts Hcl. *)
+(*     indNow' Hindt env i j. *)
+(*     indNow' Hindt1 env i j. *)
+(*   - intros * Hindt * Hindt1 * Hcl * Hlen; simpl in *; inverts Hcl. *)
+(*     indNow' Hindt env i j. *)
+(*     indNow' Hindt1 env i j. *)
+(*   - intros * Hindt * Hcl * Hlen; simpl in *; inverts Hcl. *)
+(*     indNow' Hindt env i j. *)
+(*   - intros * Hindt * Hindt1 * Hcl * Hlen; simpl in *; inverts Hcl. *)
+(*     indNow' Hindt env i j. *)
+(*     indNow' Hindt1 env i j. *)
+(*   - intros * Hindt * Hindt1 * Hindt2 * Hcl * Hlen; simpl in *; inverts Hcl. *)
+(*     indNow' Hindt env i j. *)
+(*     indLater' Hindt1 env i j. *)
+(*     indLater' Hindt2 env i j. *)
+(*   - intros * Hindt * Hcl * Hlen; simpl in *; inverts Hcl. *)
+(*     indNow' Hindt env i j. *)
+(*   - intros * Hindt * Hindt1 * Hcl * Hlen; simpl in *; inverts Hcl. *)
+(*     indNow' Hindt env i j. *)
+(*     indNow' Hindt1 env i j. *)
+(* Qed. *)
+(* (*   (*   assert (exists T', dms_subst_all env d. *) *) *)
+(* (*   (*   lets ?: Hind ___; eauto. *) *) *)
+(* (*   (*   rewrite Hind. *) *) *)
+(* (*   (*   case_match. *) *) *)
+(* (*   (* inverse HenvCl; intuition eauto using index_Forall)]. *) *) *)
+
+(* Lemma subst_all_success: *)
+(*   forall T, forall i env, forall j, closed i j T -> length env = j -> exists T', subst_all env T = Some T'. *)
+(* Proof. *)
+(*   apply subst_all_success_rec. *)
+(* Qed. *)
+
+(*   (* induction env. *) *)
+(*   (* - admit. *) *)
+(*   (* - intros * HenvCl * Hcl Hlen; *) *)
+(*   (*   simpl in *; subst. *) *)
+(*   (*   inverse HenvCl. *) *)
+
+(*   (* intros HenvCL. *) *)
+(*   (* intros * Hcl Hlen HenvCl. gen i j. *) *)
+(*   (* induction env. admit. *) *)
+(*   (* simpl in *; subst. *) *)
+(*   (* intros * Hcl Hlen HenvCl. *) *)
+(*   (* inverse HenvCl. *) *)
+(*   (* induction v; *) *)
+(*   (* simpl in *; subst; *) *)
+(*   (*   inversion Hcl; subst; *) *)
+(*   (*   eexists; split_conj; simpl; eauto; try omega. *) *)
+(*   (* case_match. *) *)
+(*   (* admit. *) *)
+
+(* Lemma subst_all_closed_upgrade_rec: *)
+(*   (forall l j v, vr_closed l j v -> forall vx, v = vr_open j vx v) /\ *)
+(*   (forall l j T, closed l j T -> forall vx, T = open j vx T) /\ *)
+(*   (forall l j t, tm_closed l j t -> forall vx, t = tm_open j vx t) /\ *)
+(*   (forall l j d, dm_closed l j d -> forall vx, d = dm_open j vx d) /\ *)
+(*   (forall l j ds, dms_closed l j ds -> forall vx, ds = dms_open j vx ds). *)
+(* Proof. *)
+
+(* The lemma that would be needed here is a different one. *)
+(* Lemma etp_closed: forall T k v env, *)
+(*     Forall (dms_closed 0 0) env -> *)
+(*     etp T k v env -> wf env T. *)
+(* Proof. *)
+(*   unfold etp, wf, closed_ty. *)
+(*   intros * Hcl H. *)
+(*   destruct H as (T'' & e'' & Hty & Htm & Hclosed & Hexp). *)
+(*   lets (_ & HclTh & _) : subst_all_closed_upgrade_rec. *)
+(*   lets ? : HclTh T 0 0 env. *)
+(*   (* lets (? & ? & ?) : (proj1 (proj2 subst_all_closed_upgrade_rec)) ___. *) *)
+(*   simp expr_sem in *. ev. *)
+(*   tauto. *)
+(* Qed. *)
+(* Hint Resolve etp_closed. *)
+
+Definition wf {A} (G : list A) T := closed 0 (length G) T.
+
+Program Definition etp T k e :=
+  expr_sem k T (fun k _ => vtp T k) k _ e.
+
+Lemma etp_closed: forall T k v,
+    etp T k v -> @wf ty [] T.
+Proof.
+  unfold etp; intros; simp expr_sem in *; tauto.
+Qed.
+Hint Resolve etp_closed.
+
+Program Lemma index_sigT : forall {X} vs (n : {n : id | n < length vs}),
+                       {T:X & index (proj1_sig n) vs = Some T}.
+Proof.
+  intros ? vs [n H]; induction vs; simpl in *.
+  - exfalso; inversion H.
+  - better_case_match; beq_nat; subst; eauto.
+Qed.
+
+Definition indexTot {X} (xs : list X) (n : {n : id | n < length xs}): X :=
+  projT1 (index_sigT xs n).
+
+Program Fixpoint vr_subst_all_tot i (env: list vr) (v: vr) (_ : vr_closed i (length env) v) { struct v }: vr :=
   match v with
     | VarF x => VarF x
-    | VarB x =>
-      VarB x
-      (* index x env *)
-    | VObj dms => VObj (dms_subst_all (VObj dms :: env) dms)
+    | VarB x => indexTot env x
+    | VObj dms =>
+      let dms' := dms_subst_all_tot i (VarB 0 :: env) dms _ in
+      VObj dms'
   end
-with subst_all (env: list vr) (T: ty) { struct T }: ty :=
+with subst_all_tot i (env: list vr) (T: ty) (_ : closed i (length env) T){ struct T }: ty :=
   match T with
     | TTop        => TTop
     | TBot        => TBot
-    | TSel v1 l     => TSel (vr_subst_all env v1) l
-    | TFun l T1 T2  => TFun l (subst_all env T1) (subst_all (VarB 0 :: env) T2)
-    | TMem l T1 T2  => TMem l (subst_all env T1) (subst_all env T2)
-    | TBind T1    => TBind (subst_all (VarB 0 :: env) T1)
-    | TAnd T1 T2  => TAnd (subst_all env T1) (subst_all env T2)
-    | TOr T1 T2   => TOr (subst_all env T1) (subst_all env T2)
+    | TSel v1 l     =>
+      let v1' := vr_subst_all_tot i env v1 _ in
+      TSel v1' l
+    | TFun l T1 T2  =>
+      let T1' := subst_all_tot i env T1 _ in
+      let T2' := subst_all_tot i (VarB 0 :: env) T2 _ in
+      TFun l T1' T2'
+    | TMem l T1 T2  =>
+      let T1' := subst_all_tot i env T1 _ in
+      let T2' := subst_all_tot i env T2 _ in
+      TMem l T1' T2'
+    | TBind T1    =>
+      let T1' := subst_all_tot i (VarB 0 :: env) T1 _ in
+      TBind T1'
+    | TAnd T1 T2  =>
+      let T1' := subst_all_tot i env T1 _ in
+      let T2' := subst_all_tot i env T2 _ in
+      TAnd T1' T2'
+    | TOr T1 T2   =>
+      let T1' := subst_all_tot i env T1 _ in
+      let T2' := subst_all_tot i env T2 _ in
+      TOr T1' T2'
   end
-with tm_subst_all (env: list vr) (t: tm) { struct t }: tm :=
+with tm_subst_all_tot i (env: list vr) (t: tm) (_ : tm_closed i (length env) t) { struct t }: tm :=
    match t with
-     | tvar v => tvar (vr_subst_all env v)
-     | tapp t1 l t2 => tapp (tm_subst_all env t1) l (tm_subst_all env t2)
+     | tvar v => let v' := vr_subst_all_tot i env v _ in tvar v'
+     | tapp t1 l t2 =>
+       let t1' := tm_subst_all_tot i env t1 _ in
+       let t2' := tm_subst_all_tot i env t2 _ in
+       tapp t1' l t2'
    end
-with dm_subst_all (env: list vr) (d: dm) { struct d }: dm :=
+with dm_subst_all_tot i (env: list vr) (d: dm) (_ : dm_closed i (length env) d) { struct d }: dm :=
    match d with
-     | dfun T1 T2 t2 => dfun (subst_all env T1) (subst_all (VarB 0 :: env) T2) (tm_subst_all (VarB 0 :: env) t2)
-     | dty T1 => dty (subst_all env T1)
+     | dfun T1 T2 t2 =>
+       let T1' := subst_all_tot i env T1 _ in
+       let T2' := subst_all_tot i (VarB 0 :: env) T2 _ in
+       let t2' := tm_subst_all_tot i (VarB 0 :: env) t2 _ in
+       dfun T1' T2' t2'
+     | dty T1 =>
+       let T1' := subst_all_tot i env T1 _ in
+       dty T1'
    end
-with dms_subst_all (env: list vr) (ds: dms) { struct ds }: dms :=
+with dms_subst_all_tot i (env: list vr) (ds: dms) (_ : dms_closed i (length env) ds) { struct ds }: dms :=
    match ds with
      | dnil => dnil
-     | dcons d ds => dcons (dm_subst_all env d) (dms_subst_all env ds)
+     | dcons d ds =>
+       let d'  := dm_subst_all_tot i env d _ in
+       let ds' := dms_subst_all_tot i env ds _ in
+       dcons d' ds'
    end.
+Solve All Obligations with program_simpl; inverts H; auto.
 
-(* Program Definition etp T k e env := *)
-(*   @expr_sem k T (fun k _ => vtp T k) k _ env e env. *)
-(* (* Semantic typing *) *)
-(* Definition sem_type (G : tenv) (T : ty) (e: tm) := *)
-(*   wf G T /\ *)
+(* Scheme vr_mut_type := Induction for vr Sort Set *)
+(* with   ty_mut_type := Induction for ty Sort Set *)
+(* with   tm_mut_type := Induction for tm Sort Set *)
+(* with   dm_mut_type := Induction for dm Sort Set *)
+(* with   dms_mut_type := Induction for dms Sort Set. *)
+(* Combined Scheme syntax_mut_typeind from vr_mut_type, ty_mut_type, tm_mut_type, dm_mut_type, dms_mut_type. *)
+
+(* Lemma subst_all_success_rec_sig: *)
+(*   (forall v, forall i env, forall j, vr_closed i j v -> length env = j -> { v' | vr_subst_all env v = Some v'}) * *)
+(*   (forall T, forall i env, forall j, closed i j T -> length env = j -> { T' | subst_all env T = Some T'}) * *)
+(*   (forall t, forall i env, forall j, tm_closed i j t -> length env = j -> { t' | tm_subst_all env t = Some t'}) * *)
+(*   (forall dm, forall i env, forall j, dm_closed i j dm -> length env = j -> { dm' | dm_subst_all env dm = Some dm'}) * *)
+(*   (forall T, forall i env, forall j, dms_closed i j T -> length env = j -> { dms' | dms_subst_all env T = Some dms'}). *)
+(* Proof. *)
+(*   apply syntax_mutind. *)
+(*   Abort. *)
+
+(* Program Definition subst_all_tot (env: venv) T (HclT: closed 0 (length env) T) := *)
+(*   let '(ex_intro _ A B) := (subst_all_success T 0 (map VObj env) (length env) HclT eq_refl) *)
+(*   in A. *)
+(* Check subst_all_tot. *)
+
+Hint Rewrite map_length.
+
+Program Definition vtpEnvCore T k v env (HwfT : wf env T) (HwfV : tm_closed 0 (length env) v) :=
+  let venv := map VObj env in
+  vtp (subst_all_tot 0 venv T _) k (tm_subst_all_tot 0 venv v _).
+Solve Obligations with program_simpl; rewrite map_length; auto.
+
+Program Definition vtpEnv T k v env :=
+  { HwfT : wf env T |
+    { HwfV : tm_closed 0 (length env) v | vtpEnvCore T k v env _ _ }}.
+
+Lemma vtpEnv_closed:
+  forall T k v env, vtpEnv T k v env -> wf env T.
+Proof. unfold vtpEnv, wf, closed_ty; program_simpl. Qed.
+Hint Resolve vtpEnv_closed.
+
+(* Definition vtpEnv T k v env := *)
+(*   let venv := map VObj env in *)
+(*   let T' := subst_all venv T in *)
+(*   let v' := tm_subst_all venv v in *)
+(*   closed_ty 0 (length env) T /\ *)
+(*   exists T'' v'', *)
+(*     T' = Some T'' /\ *)
+(*     v' = Some v'' /\ *)
+(*     vtp T'' k v''. *)
+
+Set Transparent Obligations. (* XXX only for one unfold later, check if really needed. *)
+
+Program Definition etpEnvCore T k e env (HwfT : wf env T) (HwfE : tm_closed 0 (length env) e) :=
+  let venv := map VObj env in
+  let T' := subst_all_tot 0 venv T _ in
+  expr_sem k T' (fun k _ => vtp T' k) k _ (tm_subst_all_tot 0 venv e _).
+
+Solve Obligations with program_simpl; rewrite map_length; auto.
+
+Program Definition etpEnv T k e env :=
+  { HwfT : wf env T |
+    { HwfE : tm_closed 0 (length env) e | etpEnvCore T k e env _ _ }}.
+
+Lemma etpEnv_closed: forall T k v env,
+    etpEnv T k v env -> wf env T.
+Proof. unfold etpEnv, wf; program_simpl. Qed.
+Hint Resolve etpEnv_closed.
+
+(* Semantic typing *)
+Program Definition sem_type (G : tenv) (T : ty) (e: tm) :=
+  { HwfT : wf G T | { HwfE : tm_closed 0 (length G) e |
+      forall k env (Henv: R_env k env G), etpEnvCore T k e env _ _ }}.
+Solve Obligations with program_simpl; unfold wf in *; erewrite wf_length in *; eauto.
+
+Program Definition sem_subtype (G : tenv) (T1 T2: ty) :=
+  { HwfT1 : wf G T1 |
+    { HwfT2 : wf G T2 |
+      forall e (HwfE : tm_closed 0 (length G) e),
+      forall k env (Henv : R_env k env G),
+        etpEnvCore T1 k e env _ _ -> etpEnvCore T2 k e env _ _ }}.
+Solve Obligations with program_simpl; unfold wf in *; erewrite wf_length in *; eauto.
+
+Program Definition sem_vl_subtype (G : tenv) (T1 T2: ty) :=
+  { HwfT1 : wf G T1 |
+    { HwfT2 : wf G T2 |
+      forall e (HwfE : tm_closed 0 (length G) e),
+      forall k env (Henv : R_env k env G),
+        vtpEnvCore T1 k e env _ _ -> vtpEnvCore T2 k e env _ _ }}.
+Solve Obligations with program_simpl; unfold wf in *; erewrite wf_length in *; eauto.
+
+(* Definition sem_subtype (G : tenv) (T1 T2: ty) := *)
+(*   wf G T1 /\ *)
+(*   wf G T2 /\ *)
 (*   forall k env, *)
 (*     R_env k env G -> *)
-(*     etp T k e. *)
+(*     forall e, etpEnv T1 k e env -> etpEnv T2 k e env. *)
+
+(* Definition sem_vl_subtype (G : tenv) (T1 T2: ty) := *)
+(*   wf G T1 /\ *)
+(*   wf G T2 /\ *)
+(*   forall k env, *)
+(*     R_env k env G -> *)
+(*     forall v, *)
+(*       vtpEnv T1 k v env -> vtpEnv T2 k v env. *)
+
+Lemma sem_type_closed : forall G T e,
+    sem_type G T e -> wf G T.
+Proof. unfold sem_type; program_simpl. Qed.
+
+Lemma sem_subtype_closed1 : forall G T1 T2,
+    sem_subtype G T1 T2 -> wf G T1.
+Proof. unfold sem_subtype; program_simpl. Qed.
+
+Lemma sem_subtype_closed2 : forall G T1 T2,
+    sem_subtype G T1 T2 -> wf G T2.
+Proof. unfold sem_subtype; program_simpl. Qed.
+
+Lemma sem_vl_subtype_closed1 : forall G T1 T2,
+    sem_vl_subtype G T1 T2 -> wf G T1.
+Proof. unfold sem_vl_subtype; program_simpl. Qed.
+
+Lemma sem_vl_subtype_closed2 : forall G T1 T2,
+    sem_vl_subtype G T1 T2 -> wf G T2.
+Proof. unfold sem_vl_subtype; program_simpl. Qed.
+
+Hint Resolve sem_type_closed
+     sem_subtype_closed1
+     sem_subtype_closed2
+     sem_vl_subtype_closed1
+     sem_vl_subtype_closed2.
+Hint Resolve wf_length.
+
+(* Lemma closed_subst_success: forall T env, *)
+(*     (closed_ty 0 (length env) T) -> *)
+(*     exists T1, subst_all env T = Some T1. *)
+(* Admitted. *)
+
+(* Write lemmas to get rid of all the extra side conditions and get to the meat. *)
+Lemma vl_subtype_to_subtype : forall G T1 T2,
+    sem_vl_subtype G T1 T2 -> sem_subtype G T1 T2.
+Proof.
+  unfold sem_subtype, sem_vl_subtype, wf.
+  program_simpl.
+  repeat match goal with
+         | H: ?P |- { H : ?P | ?Q } => exists H
+         end.
+  intros.
+  unfold etpEnvCore in *; simp expr_sem in *.
+  ev; split_conj; intros.
+  - admit.
+  - exists v.
+    unfold vtpEnvCore in *.
+    (* unfold etpEnvCore_obligation_1 in *. *)
+    intuition eauto.
+    (* XXX Reprove subst_all_closed_upgrade_rec for subst_all_tot. Then, modify
+    vtp to ensure it only holds for closed terms, prove it, lift that proof to
+    R_env, then try again (or maybe rather move the hard work in vtp_etp and etp_vtp lemmas). *)
+
+(*   - intros. *)
+(*   vtp, etpEnvCore, vtpEnvCore; simp val_type. *)
+(*   unfold etpEnv in *. *)
+(*   Transparent expr_sem. *)
+(*   unfold expr_sem. *)
+(*   Opaque expr_sem. *)
+(*   intros * (? & ? & Himpl); split_conj; eauto. intros * Henv * (? & ?). *)
+
+(*   ev; split_conj; *)
+(*     replace (length G) with (length env) in * by eauto; *)
+(*     eauto. *)
+(*   lets (? & ?): closed_subst_success T2 (map VObj env) ___; *)
+(*   try rewrite map_length; eauto. *)
+(*   do 2 eexists; split_conj; eauto. *)
+(*   admit. *)
+(*   eauto. *)
+(*   (* info_eauto. *) *)
+(*   (* info_eauto. *) *)
+(*   (* info_eauto. *) *)
+
+(*   (* intuition info_eauto. *) *)
+(*   (* - admit. *) *)
+(*   (* - lets (? & ?) : H5 v j ___; eauto. eapply H9. *) *)
+(*   (*   eauto. *) *)
+
+(*   (* simp expr_sem in *; ev. *) *)
+(*   (* lets ? : Himpl Henv e ___; intuition eauto; repeat eexists. *) *)
+(*   (* eauto. *) *)
+(*   (* eauto. *) *)
+(* Admitted. *)
+(* Hint Resolve vl_subtype_to_subtype. *)
+
+Abort.
